Cleanup LList example

examples/steel/arraystructs/LList.fst
@@ -135,87 +135,6 @@ let fold_pts_to_llist (#opened:inames) (p:ptr node node) (l:cells)
      pts_to_llist_tl l pts_to_llist)
     (p `pts_to_llist` l)
 
-(*
-unfold let f (x:option 'a): Tot prop = x == None #'a
-let good #a: squash ((None #a == None #a) == (f (None #a))) = ()
-
-let g (x:'a): Tot prop = x == x
-let good : squash ((None #int == None #int) == (g (None #int))) = ()
-
-let g (x:option int): Tot prop = x == None #int
-let bad : squash ((None #int == None #int) == (g (None #int))) = ()
-
-let g (x:option 'a): Tot prop = x == None #'a
-let bad #a: squash ((None #a == None #a) == (g (None #a))) =
-  assert_norm ((None #a == None #a) == (g (None #a)))
-
-let f (x:'a): Tot prop = x == x
-let good #a: squash ((3 == 3) == (f 3)) = ()
-
-let f (l:list 'a): Tot prop
-= (l == [])
-let bad #a: squash (([] #a == [] #a) == (f ([] #a))) = ()
-
-let f (l:list 'a): Tot prop
-= (l == [])
-let aux' #a =
-  assert_norm (
-    ([] #a == [])
-    ==
-    f ([] #a))
-
-let aux' #a =
-  assert_norm (
-    (let l = [] #a in
-    ((l == [])))
-    ==
-    f ([] #a))
-    
-let f (l:cells)
-: Tot vprop
-= vpure (l == [])
-
-let aux' (p: ptr node node) =
-  assert_norm (
-    (let l = [] #cell in
-    (LList.vpure (l == [])))
-    ==
-    f ([] #cell))
-
-let pts_to_llist' (p:ptr node node) (l:cells)
-: Tot vprop (decreases (List.length l))
-= vpure (p == nullptr <==> l == [])
-
-let aux' (p: ptr node node) =
-  assert_norm (
-    (let l = [] #cell in
-    (LList.vpure (p == Steel.C.Ptr.nullptr <==> l == [])))
-    ==
-    pts_to_llist' p ([] #cell))
-
-let aux' (p: ptr node node) =
-  assert_norm(
-    (let l = [] #cell in
-    Steel.Effect.Common.star (Steel.Effect.Common.star (LList.vpure (p == Steel.C.Ptr.nullptr <==>
-                l == []))
-          (Steel.C.Ptr.pts_to_or_null p ListNode.node_pcm (LList.hd_node l)))
-      (LList.pts_to_llist_tl l LList.pts_to_llist))
-    ==
-    pts_to_llist p ([] #cell))
-
-let aux p =
-    assert_norm (
-( vpure (p == nullptr <==> [] #cell == []) `star`
- pts_to_or_null p node_pcm (hd_node ([] #cell)) `star`
- pts_to_llist_tl ([] #cell) pts_to_llist)
-     ==
-    (p `pts_to_llist` [] #cell))
-    
-//  vpure (p == nullptr <==> l == []) `star`
-//  pts_to_or_null p node_pcm (hd_node l) `star`
-//  pts_to_llist_tl l pts_to_llist
-*)
-
 let intro_pts_to_llist_nil #opened p
 : SteelGhost unit opened 
     emp
@@ -348,45 +267,6 @@ let nontrivial_fact_about_mk_node value next
 : Lemma (Ghost.reveal (mk_node (some value) (some next)) =!= one node_pcm)
 = ()
 
-(*
-assume val intro_pts_to_llist_cons' : #opened:inames ->
-      p: ptr node ->
-      value: int ->
-      next: ptr node ->
-      l: Ghost.erased cells
-    -> Steel.Effect.Atomic.SteelGhostT unit
-        opened
-        (star (pts_to p node_pcm (mk_node (some (Ghost.hide value)) (some (Ghost.hide next))))
-	  (pts_to_llist next l))
-        (fun _ ->
-            pts_to_llist p
-              (Ghost.hide (FStar.Pervasives.Native.Mktuple2 value next :: Ghost.reveal l)))
-
-assume val addr_of_value
-  (#value:Ghost.erased (option int))
-  (#next:Ghost.erased (option (Steel.C.Ptr.ptr node node)))
-  (p: Steel.C.Ptr.ptr node node)
-: Steel (Steel.C.Ptr.ptr node (option int))
-    (pts_to p node_pcm (mk_node value next))
-    (fun q ->
-       (pts_to p node_pcm (mk_node none next)) `star`
-       (pts_to q opt_pcm value))
-    (requires (fun _ -> True))
-    (ensures (fun _ q _ -> ptr_focused q p _value))
-
-assume val unaddr_of_value
-  (#value:Ghost.erased (option int))
-  (#next:Ghost.erased (option (Steel.C.Ptr.ptr node node)))
-  (p: Steel.C.Ptr.ptr node node)
-  (q: Steel.C.Ptr.ptr node (option int))
-: Steel unit
-    ((pts_to p node_pcm (mk_node none next)) `star`
-     (pts_to q opt_pcm value))
-    (fun q -> pts_to p node_pcm (mk_node value next))
-    (requires (fun _ -> ptr_focused q p _value))
-    (ensures (fun _ _ _ -> True))
-    *)
-
 val is_empty
   (#l: Ghost.erased cells) (p: ptr node)
 : Steel bool
@@ -405,7 +285,7 @@ val set_first (p:ptr node) (l:Ghost.erased cells) (value:int)
     (p `pts_to_llist` l)
     (fun _ -> p `pts_to_llist` cells_set_hd value l)
 
-assume val intro_pts_to_llist_cons' : #opened:inames ->
+val intro_pts_to_llist_cons' : #opened:inames ->
       p: ptr node ->
       value: int ->
       next: ptr node ->
@@ -418,6 +298,25 @@ assume val intro_pts_to_llist_cons' : #opened:inames ->
             pts_to_llist p
               (Ghost.hide (FStar.Pervasives.Native.Mktuple2 value next :: Ghost.reveal l)))
 
+let intro_pts_to_llist_cons' p value next l = 
+  intro_pts_to_llist_cons p
+    (mk_node (some (Ghost.hide value)) (some (Ghost.hide next))) 
+    value next l
+
+(* TODO move to Steel.C.Ptr? *)
+val intro_pts_to'
+  (#pb: pcm 'b) (#v: Ghost.erased 'b)
+  (r: ref 'a pb) (p: Steel.C.Ptr.ptr 'a 'b)
+: Steel unit
+    (r `R.pts_to` v)
+    (fun _ -> pts_to p pb v)
+    (requires fun _ -> p == vptr r)
+    (ensures fun _ _ _ -> True)
+
+let intro_pts_to' r p =
+  let p' = intro_pts_to r in
+  change_equal_slprop (pts_to p' _ _) (pts_to p _ _)
+
 let set_first p l new_value =
   let b = is_empty p in
   if b then begin
@@ -429,194 +328,7 @@ let set_first p l new_value =
     let r_value = addr_of_value r in
     r_value `opt_write` new_value;
     unaddr_of_value r r_value;
-    let p' = intro_pts_to r in
-    assert (p == p');
-    change_equal_slprop (pts_to p' _ _) (pts_to p _ _);
+    intro_pts_to' r p;
     intro_pts_to_llist_cons' p new_value res.next res.tl;
     return ()
   end
-
-(*
-let rec cells_set_nth (n:nat) (value:int) (l:cells) : Tot cells (decreases n) =
-  if n = 0 then cells_set_hd value l
-  else match l with
-  | [] -> []
-  | hd :: tl -> hd :: cells_set_nth (n - 1) value tl
-
-let rec cells_set_nth_nil n value
-: Lemma (ensures cells_set_nth n value [] == []) (decreases n)
-= if n = 0 then () else cells_set_nth_nil (n - 1) value
-
-let llist_setter (n:nat) =
-  p:ptr node -> l:Ghost.erased cells -> value:int ->
-  SteelT unit
-    (p `pts_to_llist` l)
-    (fun _ -> p `pts_to_llist` cells_set_nth n value l)
-
-let llist_set_zero: llist_setter 0 = set_hd
-
-// TODO set_hd: can make helper function is_empty to check whether list is empty or not
-
-let aux n value l = cells_set_nth (n + 1) value l
-
-let aux n (ih: llist_setter n) (p: ptr node) (l: Ghost.erased cells) (new_value: int)
-: SteelT unit
-    (p `pts_to_llist` l)
-    (fun _ -> p `pts_to_llist` cells_set_nth (n + 1) new_value l)
-= unfold_pts_to_llist p l;
-  let b = is_null p in
-  fold_pts_to_llist p l;
-  assume (b == false);
-  //if b then begin
-  //  pts_to_llist_nullptr p l;
-  //  cells_set_nth_nil (n + 1) new_value;
-  //  return ()
-  //end else begin
-    let res = elim_pts_to_llist_cons p l in
-    let r = elim_pts_to p in
-    let r_next = addr_of_next r in
-    let q = opt_read r_next in
-    unaddr_of_next r r_next;
-    assert (q == res.next);
-    change_equal_slprop (res.next `pts_to_llist` _) (q `pts_to_llist` _);
-    ih q res.tl new_value;
-    //let p' = intro_pts_to r in
-    //change_equal_slprop (pts_to p' node_pcm _) (pts_to p node_pcm _);
-    //intro_pts_to_llist_cons p
-    //  (mk_node (some (Ghost.hide new_value)) (some (Ghost.hide res.next)))
-    //  new_value res.next res.tl;
-    sladmit();
-    return ()
-  //end
-
-  // assume (Some? p);
-  // // match p with
-  // // | None ->
-  // //   pts_to_llist_nullptr p l;
-  // //   cells_set_nth_nil (n + 1) value;
-  // //   change_equal_slprop
-  // //     (None `pts_to_llist` [])
-  // //     (p `pts_to_llist` cells_set_nth (n + 1) value l);
-  // //   return ()
-  // // | Some r ->
-  // let Some r = p in
-  //   let res = pts_to_llist_some p l in
-  //   let value: Ghost.erased int = Ghost.hide res.value in
-  //   let next: Ghost.erased ptr = Ghost.hide res.next in
-  //   let tl: Ghost.erased cells = Ghost.hide res.tl in
-  //   //let value: Ghost.erased int = Ghost.hide (fst value_next_tl) in
-  //   //let next: Ghost.erased ptr = Ghost.hide (fst (snd value_next_tl)) in
-  //   //let tl: Ghost.erased cells = Ghost.hide (snd (snd value_next_tl)) in
-  //   change_equal_slprop (p `pts_to_llist` l)
-  //     (Some r `pts_to_llist`
-  //      Ghost.hide ((Ghost.reveal value, Ghost.reveal next) :: Ghost.reveal tl));
-  //   let r' = elim_llist_cons (Some r) (Ghost.reveal value) (Ghost.reveal next) (Ghost.reveal tl) in
-  //   let r: ref node node_pcm = r in
-  //   change_equal_slprop (Ghost.reveal r' `pts_to` mk_node (some value) (some next))
-  //     (r `pts_to` mk_node (some value) (some next));
-  //   let r_next = addr_of_next r in
-  //   let q: ptr = opt_read r_next in
-  //   assert (q == Ghost.reveal next);
-  //   unaddr_of_next r r_next;
-  //   change_equal_slprop (Ghost.reveal next `pts_to_llist` _) (q `pts_to_llist` _);
-  //   ih q tl new_value;
-  //   change_equal_slprop (q `pts_to_llist` _) (Ghost.reveal next `pts_to_llist` _);
-  //   intro_llist_cons r (Ghost.reveal value) (Ghost.reveal next) _;
-//// val intro_llist_cons
-////   (#opened:inames) (r: ref node node_pcm)
-////   (value: int) (next: ptr)
-////   (tl: cells)
-//// : SteelGhostT unit opened
-////     ((r `pts_to` mk_node (some value) (some next)) `star` (next `pts_to_llist` tl))
-////     (fun _ -> Some r `pts_to_llist` ((value, next)::tl))
-  //   sladmit(); return ()
-  //   // //assert (Ghost.reveal r' == r);
-  //   // //slassert (Ghost.reveal r' `pts_to` mk_node (some value) (some next));
-  //   // let r_value = addr_of_value r in
-  //   // r_value `opt_write` new_value;
-  //   // unaddr_of_value r r_value;
-  //   // intro_llist_cons r new_value next tl;
-  //   // //change_equal_slprop (Ghost.reveal r' `pts_to` mk_node _ _) (r `pts_to` mk_node _ _);
-  //   // //sladmit(); return ()
-  //   // return ()
-  // let set_hd p l new_value =
-
-let llist_set_succ n (ih: llist_setter n): llist_setter (n + 1) =
-  let aux (p: ptr) (l: Ghost.erased cells) (value: int)
-  : SteelT unit
-      (p `pts_to_llist` l)
-      (fun _ -> p `pts_to_llist` cells_set_nth (n + 1) value l)
-  = assume (Some? p);
-    // match p with
-    // | None ->
-    //   pts_to_llist_nullptr p l;
-    //   cells_set_nth_nil (n + 1) value;
-    //   change_equal_slprop
-    //     (None `pts_to_llist` [])
-    //     (p `pts_to_llist` cells_set_nth (n + 1) value l);
-    //   return ()
-    // | Some r ->
-    let Some r = p in
-      let res = pts_to_llist_some p l in
-      let value: Ghost.erased int = Ghost.hide res.value in
-      let next: Ghost.erased ptr = Ghost.hide res.next in
-      let tl: Ghost.erased cells = Ghost.hide res.tl in
-      //let value: Ghost.erased int = Ghost.hide (fst value_next_tl) in
-      //let next: Ghost.erased ptr = Ghost.hide (fst (snd value_next_tl)) in
-      //let tl: Ghost.erased cells = Ghost.hide (snd (snd value_next_tl)) in
-      change_equal_slprop (p `pts_to_llist` l)
-        (Some r `pts_to_llist`
-         Ghost.hide ((Ghost.reveal value, Ghost.reveal next) :: Ghost.reveal tl));
-      let r' = elim_llist_cons (Some r) (Ghost.reveal value) (Ghost.reveal next) (Ghost.reveal tl) in
-      let r: ref node node_pcm = r in
-      change_equal_slprop (Ghost.reveal r' `pts_to` mk_node (some value) (some next))
-        (r `pts_to` mk_node (some value) (some next));
-      let r_next = addr_of_next r in
-      let q: ptr = opt_read r_next in
-      unaddr_of_next r r_next;
-      //ih q tl value;
-      sladmit(); return ()
-      // //assert (Ghost.reveal r' == r);
-      // //slassert (Ghost.reveal r' `pts_to` mk_node (some value) (some next));
-      // let r_value = addr_of_value r in
-      // r_value `opt_write` new_value;
-      // unaddr_of_value r r_value;
-      // intro_llist_cons r new_value next tl;
-      // //change_equal_slprop (Ghost.reveal r' `pts_to` mk_node _ _) (r `pts_to` mk_node _ _);
-      // //sladmit(); return ()
-      // return ()
-  in aux
-
-// TODO look at #2319, construct module of (possibly null) pointers
-// (define pts_to_or_null; can compare against null only if points to non-unit)
-
-// Mutate the kth element of a list (of fixed k)
-// 
-// t k = type of functions that mutate kth element of a list
-// 
-// set_zero : Tot (t 0)
-// set_succ : t k -> Tot (t (k + 1))
-//
-// let rec set k .. : Steel _ = 
-// let rec set k .. : Tot (.. -> Steel _) = 
-
-(*
-val pop (#a:Type) (ptr:t a) (l:list (cell a){Cons? l})
-  : Steel a
-          (llist ptr l)
-          (fun _ -> llist (next (L.hd l)) (L.tl l))
-          (requires fun _ -> True)
-          (ensures fun _ x _ -> x == data (L.hd l))
-
-let pop #a ptr l =
-  let hd = L.hd l in
-  let tl = L.tl l in
-  rewrite_slprop (llist ptr l) (llist ptr (hd::tl)) (fun _ -> ());
-  elim_llist_cons ptr hd tl;
-  let c = read_pt ptr in
-  let n = next hd in
-  free_pt ptr;
-  rewrite_slprop (llist (next hd) tl) (llist (next (L.hd l)) (L.tl l)) (fun _ -> ());
-  return (data c)
-*)
-*)
